CartesianClosed.v
@@ -1,0 +1,51 @@
+Add Rec LoadPath "/home/zeimer/Code/Coq".
+
+Require Export Cat.
+Require Import InitTerm.
+Require Import BinProdCoprod.
+Require Import Exponential.
+
+Class cartesian_closed (C : Cat) : Type :=
+{
+    ccc_term :> has_term C;
+    ccc_prod :> has_products C;
+    ccc_exp :> has_exponentials C
+}.
+
+Arguments term [C] [has_term].
+Arguments delete [C] [has_term] _.
+Arguments diag [C] [has_products] _ _ _ _ _.
+
+Theorem id_unique_left' : forall (C : Cat) (X Y : Ob C)
+    (f : Hom X Y) (g : Hom Y X), f .> g .> f == f -> f .> g == id X.
+Proof.
+  intros. apply id_unique_left. intros.
+
+Theorem prod_term_iso : forall (C : Cat) (X : Ob C)
+    (ht : has_term C) (hp : has_products C),
+        prodOb term X ~ X.
+Proof.
+  symmetry. (*destruct ht, hp*) intros; red; simpl.
+  pose (f := diag term X X (delete X) (id X)).
+  exists f; red. exists (proj2 term X). unfold f.
+  destruct (is_product term X X (delete X) (id X)) as [[H1 H2] H3].
+  split.
+    rewrite <- H2. reflexivity.
+    assert (diag term X X (delete X) (id X) .> proj2 term X
+      .> diag term X X (delete X) (id X) ==
+      diag term X X (delete X) (id X)).
+        rewrite <- H2, id_left. reflexivity.
+Check id_unique_left. apply id_unique_left. intros.
+    rewrite comp_assoc. 
+    destruct (is_product term X (prodOb term X) (delete _) (proj2 term X)).
+      destruct H0. specialize (H4 (id _)). cat.
+      assert (delete (prodOb term X) == proj1 term X).
+      destruct ht. simpl in *. rewrite <- is_terminal. reflexivity.
+      
+      destruct (is_terminal (prodOb term X) (proj1 term X)).
+
+
+
+    rewrite <- ProductFunctor_fmap_pres_id.
+      unfold ProductFunctor_fmap.
+      
